extracted/Extractor.v
@@ -1,4 +1,5 @@
 From Reactive.Translations Require LustreAstToLustre LustreOrderedToImp LustreOrdering.
+From Reactive.Props Require Axioms.
 
 From Corelib Require Extraction.
 From Stdlib Require Import ExtrOcamlBasic ExtrOcamlNatInt ExtrOcamlNativeString.
@@ -7,7 +8,7 @@ From Stdlib Require Import ExtrOcamlBasic ExtrOcamlNatInt ExtrOcamlNativeString.
 
 Extract Constant String.compare => "StringImpl.compare".
 Extract Constant LustreOrdering.node_ordering => "Ordered.node_ordering".
-Extract Constant Base.ABORT_FIXME => "Abort.aBORT_FIXME".
+Extract Constant Axioms.ABORT_FIXME => "Abort.aBORT_FIXME".
 
 Separate Extraction
   LustreOrdering.translate_node
